LibHypsNaming.v
@@ -1,0 +1,144 @@
+Require Import ZArith.
+
+(** * A general renaming scheme for hypothesis *)
+
+(** ** The default fallback renaming strategy 
+  This is used if the user-defined renaing scheme fails to give a name
+  to a hypothesis. [th] is the type of the hypothesis. *)
+Ltac fallback_rename_hyp th :=
+  match th with
+    | true = beq_nat _ _ => fresh "hbeqnat_true"
+    | beq_nat _ _ = true => fresh "hbeqnat_true"
+    | false = beq_nat _ _ => fresh "hbeqnat_false"
+    | beq_nat _ _ = false => fresh "hbeqnat_false"
+    | beq_nat _ _ = _ => fresh "hbeqnat"
+    | Zeq_bool _ _ = true => fresh "heq_Z_true"
+    | Zeq_bool _ _ = false => fresh "heq_Z_false"
+    | true = Zeq_bool _ _ => fresh "heq_Z_true"
+    | false = Zeq_bool _ _ => fresh "heq_Z_false"
+    | Zeq_bool _ _ = _ => fresh "heq_Z"
+    | _ = Zeq_bool _ _ => fresh "heq_Z"
+    | @eq bool _ true => fresh "heq_bool_true"
+    | @eq bool _ false => fresh "heq_bool_false"
+    | @eq bool true _ => fresh "heq_bool_true"
+    | @eq bool false _ => fresh "heq_bool_false"
+    | @eq bool _ _ => fresh "heq_bool"
+    | @eq nat _ true => fresh "heq_nat_true"
+    | @eq nat _ false => fresh "heq_nat_false"
+    | @eq nat true _ => fresh "heq_nat_true"
+    | @eq nat false _ => fresh "heq_nat_false"
+    | @eq nat _ _ => fresh "heq_nat"
+    | _ <> _ => fresh "hneq"
+    | _ = _ => fresh "heq"
+  end.
+
+(** ** The custom renaming tactic
+  This tactic should be redefined in each module, it should return a
+  fresh name build from the type of (hypothesis) h. It should fail if
+  no name is found, so that the fallback scheme is called.
+
+  Typical use:
+
+<<
+Ltac my_rename_hyp th :=
+  match th with
+    | (ind1 _ _ _ _) => fresh "h_ind1"
+    | (ind2 _ _) => fresh "h_ind2"
+    | f1 _ _ = true => fresh "hf_eq_true"
+    | f1 _ _ = false => fresh "hf_eq_false"
+    | f1 _ _ = _ => fresh "hf_eq"
+    | _ => previously_defined_renaming_tac1 th
+    | _ => previously_defined_renaming_tac2 th
+  end.
+>>
+
+And then overwrite the definition of rename_hyp with this:
+
+<<Ltac rename_hyp ::= my_rename_hyp.>> *)
+Ltac rename_hyp ht := fail.
+
+(** "marks" hypothesis h of the current goal by putting id(..) on top
+   of there types. *)
+Ltac id_ify h := let th := type of h in change (id th) in h.
+
+(** Unmarking one hyp. *)
+Ltac unid H :=
+  match type of H with
+    | id ?th => change th in H
+  end.
+
+(** Unmarking all hyps *)
+Ltac unidall :=
+  repeat match goal with
+    | H: id ?th |- _ => change th in H
+  end.
+
+(** Rename (and mark) all hypothesis using the current rename_hyp
+    tactic. It does not rename hypothesis already marked (i.e. of type
+    (id _)). *)
+Ltac rename_norm :=
+  repeat match goal with
+           | H:_ |- _ =>
+             match type of H with
+               | id _ => fail 1 (** This hyp is marked, chose another one *)
+               | ?th => let newname := rename_hyp th in
+                        rename H into newname;
+                        change (id th) in newname
+               (* If the custom renaming tactic failed, then try the fallback one *)
+               | ?th => let newname := fallback_rename_hyp th in
+                        rename H into newname;
+                        change (id th) in newname
+             end
+         end.
+
+
+
+(* Mark all current hypothesis of the goal to prevent re-renaming hyps
+   when calling renaming tactics multiple times.
+
+   Typical use: mark all hyps but the one we want to destruct (say h),
+   destruct h; rename all unmarked hyps except h, unmark all hyps.
+
+   That is:
+
+   idall ; unid h; destruct h; try id_ify h; rename_norm; unidall. *)
+Ltac idall :=
+  repeat match goal with
+           | H:_ |- _ =>
+             match type of H with
+               | id _ => fail 1
+               | ?th => change (id th) in H
+             end
+         end.
+
+
+(** ** Renaming Tacticals *)
+
+(** <<!! tactic >> (resp. << !! tactic h>>) performs <<tactic>> (resp.
+    <<tactic h>>) and renames all new hypothesis. During the process
+    all previously known hypothesis (but <<h>>) are marked. It may
+    happen that this mark get in the way during the execution of
+    <<tactic>>. We might try to find a better way to mark hypothesis. *)
+Tactic Notation "!!" tactic3(T) := idall; T ; rename_norm ; unidall.
+Tactic Notation "!!" tactic3(T) constr(h) :=
+  idall; unid h; (T h) ; try id_ify h; rename_norm ; unidall.
+(* begin hide *)
+Tactic Notation "!!" tactic3(T) constr(h) constr(h2) :=
+  idall; unid h;unid h2; (T h h2) ;
+  try id_ify h;try id_ify h2; rename_norm ; unidall.
+(* end hide *)
+
+(** ** Specific redefinition of usual tactics *)
+
+(* decompose and ex and or at once. TODO: generalize. *)
+Tactic Notation "decomp" hyp(h) := !! (fun x => decompose [and ex or] x) h.
+Tactic Notation "!induction" constr(h) := !! (fun x => induction x) h.
+Tactic Notation "!functional" "induction" constr(h) :=
+   !! (functional induction h).
+Tactic Notation "!functional" "inversion" constr(h) :=
+  !! (fun x => functional inversion x) h.
+Tactic Notation "!destruct" constr(h) := !! (destruct h).
+Tactic Notation "!intros" := idall;intros;rename_norm;unidall.
+Tactic Notation "!inversion" hyp(h) := !! (inversion h;subst).
+Tactic Notation "!invclear" hyp(h) := !! (inversion h;clear h;subst).
+
